Add `Impcontrol` family.

casestudy/ImpCompCert/Impcontrol.v
@@ -4,6 +4,8 @@ family Impcontrol extends Impzero { }
 family Impcontrol.Imp {
   Inductive statement += 
      | While  (t : expression) (b : statement)   (* while (t) { b } *)
+     | Break 
+     | Continue 
 
     family Semantics {
       Inductive cont += 
@@ -21,9 +23,70 @@ family Impcontrol.Imp {
     }
 }
 
+family Impcontrol.Implightgen {
+  family S extends Imp { }
+  family T extends Implight { }
+  
+  Inductive match_cont : S.Semenatics.cont -> T.Semantics.cont -> Prop := 
+    | match_Kwhile1: forall ce r s k s' a ts tk,
+      tr_if ce r Sskip Sbreak s' ->
+      tr_stmt ce s ts ->
+      match_cont ce k tk ->
+      match_cont_exp ce For_val a
+         (Csem.Kwhile1 r s k)
+         (Kseq (makeif a Sskip Sbreak)
+           (Kseq ts (Kloop1 (Ssequence s' ts) Sskip tk)))
+
+  (* Inductive match_states : S.Semantics.state -> T.Semantics.state := ... *)
+  
+  Field translate_program {
+      Case While := ...
+  }
+
+  family CorrectnessProofs {
+      Lemma translate_step:
+       forall S1 S2, S.Semantics.step S1 S2 ->
+       forall T1, match_states S1 T1 ->
+       exists T2, plus T.Semantics.step T1 T2 /\ match_states S2 T2.
+      Proof.  
+        Case While := ...     
+      Qed.
+  }
+}
+
 family Imploop.Impfrontend { 
     Inductive statement : Type +=
-       | Sloop: statement -> statement -> statement (**r infinite loop *)                               
+       | Sloop: statement -> statement -> statement (**r infinite loop *)       
+}
+
+family Imploop.Impfrontend.Semantics {
+  Inductive cont : Type += ...
+
+  Inductive step : state -> state -> Prop += 
+    | step_loop: forall f s k e le m,
+      step (State f (Sloop s) k e le m)
+        E0 (State f s (Kseq (Sloop s) k) e le m)                                          
+}
+
+family Imploop.ImpfrontendTransform { 
+  Definition translate_program := ...
+  family Proofs {
+      Lemma translate_step:
+       forall S1 S2, Source.Semantics.step S1 S2 ->
+       forall T1, match_states S1 T1 ->
+       exists T2, plus Target.Semantics.step T1 T2 /\ match_states S2 T2.
+      Proof.  
+        Case Sloop := ...     
+      Qed.
+
+
+  (*  Lemma translate_initial_states: ... Inherited *)
+   
+  (* Lemma translate_final_states: Inherited *)
+  
+  (* Theorem translate_program_correct : Inherited *)
+  
+  }                                  
 }
 
 family Imploop.Impbackend { }
